Added AST nodes to PerfExpr for node step runtmies

ironfleet/src/Dafny/Distributed/Common/Framework/Performance.s.dfy
@@ -3,41 +3,14 @@ include "Host.s.dfy"
 include "DistributedSystem.s.dfy"
 include "../Collections/Seqs.i.dfy"
 
-module Performance_s {
+abstract module Performance_s {
   import opened Collections__Seqs_i
+  import opened DS_s : DistributedSystem_s
 
-  /*
-  datatype PerformanceReport = PerfVoid | PerfZero | PerformanceReport(instructions: int, pktsDelivered: int)
-  type PerfReport = PerformanceReport
+  datatype PerfExpr = PerfStep(hstep:HostStep)| PerfVoid | PerfZero | PerfAdd(prs:multiset<PerfExpr>) | PerfMax(prs:multiset<PerfExpr>)
 
-  predicate {:axiom} PerfLe(lhs:PerfReport, rhs:PerfReport)
-    ensures lhs == PerfZero() ==> PerfLe(lhs, rhs)
-    ensures lhs == PerfVoid() ==> PerfLe(lhs, rhs)
-
-  function {:axiom} PerfMax(prs:seq<PerformanceReport>): PerformanceReport
-    ensures |prs| == 1 ==> PerfMax(prs) == prs[0]
-    ensures forall pr :: pr in prs ==> PerfLe(pr, PerfMax(prs))
-    // ensures PerfVoid() in prs ==> PerfMax(prs) == PerfVoid()
-    // ensures PerfMax(prs) == PerfMax(prs[PerfZero() := 0])
-    ensures prs == []  ==> PerfMax(prs) == PerfZero()
-
-  function {:axiom} PerfAdd(prs:multiset<PerformanceReport>) : PerformanceReport
-    ensures PerfVoid() in prs ==> PerfAdd(prs) == PerfVoid()
-    ensures PerfAdd(prs) == PerfAdd(prs[PerfZero() := 0])
-    ensures forall s:multiset<PerformanceReport> :: var p := PerfAdd(s); p in prs ==> PerfAdd(prs) == PerfAdd(prs[p := prs[p] - 1])
-
-  function {:axiom} PerfAdd2(pr1:PerformanceReport, pr2:PerformanceReport) : PerformanceReport
-    ensures PerfAdd2(pr1, pr2) == PerfAdd(multiset{pr1, pr2})
-    ensures pr1 == PerfVoid ==> PerfAdd2(pr1, pr2) == PerfVoid()
-    ensures pr2 == PerfVoid ==> PerfAdd2(pr1, pr2) == PerfVoid()
-    */
-
-  datatype PerfExpr = PerfVoid | PerfZero | PerfAdd(prs:multiset<PerfExpr>) | PerfMax(prs:multiset<PerfExpr>)
-  type PerformanceReport = PerfExpr
-  type PerfReport = PerfExpr
-
-  function {:axiom} PerfAdd2(p1:PerfExpr, p2:PerfExpr) : PerfExpr
-    ensures p1.PerfAdd? ==> PerfAdd2(p1, p2) == PerfAdd(multiset{p2} + p1.prs)
+  function PerfAdd2(p1:PerfExpr, p2:PerfExpr) : PerfExpr
+    ensures p1.PerfAdd? ==> PerfEq(PerfAdd2(p1, p2), PerfAdd(multiset{p2} + p1.prs))
   {
     PerfAdd(multiset{p1, p2})
   }
@@ -53,8 +26,8 @@ module Performance_s {
 
     // Want to establish associativity
     // PerfAdd(multiset{PerfAdd(p1), prs'}) == PerfAdd(p1 + prs')
-    ensures forall prs :: p1.PerfAdd? && PerfAdd(prs) in p1.prs && p2 == PerfAdd(p1.prs + prs - multiset{PerfAdd(prs)}) ==> PerfEq(p1, p2)
-    ensures p1.PerfAdd? ==> (forall pr :: pr in p1.prs && pr.PerfAdd? && p2 == PerfAdd(p1.prs + pr.prs - multiset{PerfAdd(pr.prs)}) ==> PerfEq(p1, p2))
+    // ensures forall prs :: p1.PerfAdd? && PerfAdd(prs) in p1.prs && p2 == PerfAdd(p1.prs + prs - multiset{PerfAdd(prs)}) ==> PerfEq(p1, p2)
+    // ensures p1.PerfAdd? ==> (forall pr :: pr in p1.prs && pr.PerfAdd? && p2 == PerfAdd(p1.prs + pr.prs - multiset{PerfAdd(pr.prs)}) ==> PerfEq(p1, p2))
 
   lemma PerfProperties()
     // ensures forall p1, p2 :: p1.PerfAdd? ==> 
