ironfleet/src/Dafny/Distributed/Protocol/Lock/PerformanceProof/Definitions.i.dfy
@@ -9,7 +9,7 @@ function PerfBoundLockHeld(epoch: int) : PerfReport
   requires 0 <= epoch
 {
   var s : multiset<PerformanceReport> := multiset{};
-  var s2 := s[GetStepRuntime(GrantStep) := epoch][GetStepRuntime(AcceptStep) := epoch];
+  var s2 := s[PerfStep(GrantStep) := epoch][PerfStep(AcceptStep) := epoch];
   PerfAdd(s2)
 }
 
@@ -17,7 +17,7 @@ function PerfBoundLockInNetwork(epoch: int) : PerfReport
   requires 0 < epoch
 {
   var s : multiset<PerformanceReport> := multiset{};
-  var s2 := s[GetStepRuntime(GrantStep) := epoch][GetStepRuntime(AcceptStep) := epoch - 1];
+  var s2 := s[PerfStep(GrantStep) := epoch][PerfStep(AcceptStep) := epoch - 1];
   PerfAdd(s2)
 }
 
@@ -32,12 +32,18 @@ lemma Test(j:int)
   var p := PerfBoundLockHeld(j);
   var p' := PerfBoundLockInNetwork(j + 1);
 
-  assert p' == PerfAdd2(p, GetStepRuntime(GrantStep));
+  var s : multiset<PerformanceReport> := multiset{};
+  var s2 := s[PerfStep(GrantStep) := j][PerfStep(AcceptStep) := j];
+  var s3 := s[PerfStep(GrantStep) := j + 1][PerfStep(AcceptStep) := j];
+
+  assert s3 == s2 + multiset{PerfStep(GrantStep)};
+
+  assert PerfEq(p', PerfAdd2(p, PerfStep(GrantStep)));
 
   var p2 := PerfBoundLockHeld(j);
   var p2' := PerfBoundLockInNetwork(j + 1);
 
-  assert p2' == PerfAdd2(p2, GetStepRuntime(AcceptStep));
+  assert p2' == PerfAdd2(p2, PerfStep(AcceptStep));
 }
 
   
