ironfleet/src/Dafny/Distributed/Protocol/Lock/PerformanceProof/TaggedGLS.i.dfy
@@ -48,7 +48,7 @@ datatype TaggedGLS_State = TaggedGLS_State(
   {
     LS_NextOneServer(UntagLS_State(tls), UntagLS_State(tls'), id, UntagLIoOpSeq(ios), hstep)
       && (var recvTime := PerfMax(multiset(GetReceivePRs(ios)) + multiset{tls.t_servers[id].pr});
-      var totalTime := PerfAdd2(recvTime, GetStepRuntime(hstep));
+      var totalTime := PerfAdd2(recvTime, PerfStep(hstep));
       tls'.t_servers[id].pr == totalTime
       )
       && (forall t_io :: t_io in ios && t_io.LIoOpSend? ==> t_io.s.msg.pr == tls'.t_servers[id].pr)
