ironfleet/src/Dafny/Distributed/Protocol/Lock/Types.i.dfy
@@ -6,7 +6,7 @@ import opened Environment_s
 import opened Native__Io_s
 
 datatype LockMessage = Transfer(transfer_epoch:int) | Locked(locked_epoch:int) | Invalid
-datatype LockStep = GrantStep | AcceptStep
+datatype LockStep = GrantStep() | AcceptStep()
 
 type LockEnvironment = LEnvironment<EndPoint, LockMessage, LockStep>
 type LockPacket = LPacket<EndPoint, LockMessage>
