ironfleet/src/Dafny/Distributed/Services/Lock/LockPerformance.s.dfy
@@ -1,0 +1,8 @@
+include "../../Impl/Lock/Host.i.dfy"
+  include "../../Common/Framework/TaggedDistributedSystem.s.dfy"
+  include "LockDistributedSystem.i.dfy"
+
+module LockPerformance_i refines Performance_s {
+  import opened DS_s = Lock_DistributedSystem_i
+
+}
