ironfleet/src/Dafny/Distributed/Services/Lock/LockTaggedDistributedSystem.i.dfy
@@ -1,9 +1,10 @@
 include "../../Impl/Lock/Host.i.dfy"
   include "../../Common/Framework/TaggedDistributedSystem.s.dfy"
   include "LockDistributedSystem.i.dfy"
+  include "LockPerformance.s.dfy"
 
 module LockTaggedDistributedSystem_i refines TaggedDistributedSystem_s {
 
-  import opened DS_s = Lock_DistributedSystem_i
+  import opened P_s = LockPerformance_i
 
 }
